formal-proofs/theories/lib/asym_rendezvous/asym_rendezvous_proof.v
@@ -2,6 +2,7 @@ From iris.base_logic.lib Require Export invariants.
 From iris.proofmode Require Import tactics.
 From iris.heap_lang Require Import proofmode notation lang.
 From iris.program_logic Require Export atomic.
+From iris.bi.lib Require Import atomic.
 Require Import SegmentQueue.lib.asym_rendezvous.asym_rendezvous_spec.
 Require Import SegmentQueue.lib.asym_rendezvous.asym_rendezvous_impl.
 
@@ -26,7 +27,7 @@ Proof. solve_inG. Qed.
 
 Section asym_rendezvous_proof.
 
-Context `{heapG Σ} `{asym_rendezvousG Σ} (N: namespace).
+Context `{heapG Σ} `{asym_rendezvousG Σ} `{interruptiblyG Σ} (N: namespace).
 
 Definition fetch_permit γ := own γ (◯ ((Excl' (), None), None)).
 
@@ -76,19 +77,27 @@ Proof.
   discriminate.
 Qed.
 
-Definition asym_rendezvous_inv P ℓ γ :=
+Definition asym_rendezvous_inv ℓ γ P :=
    (* Neither reader no writer came yet. *)
   ((own γ (● ((Excl' (), Excl' ()), None)) ∗ ℓ ↦ NONEV) ∨
    (* The writer came and left the resource, but the reader didn't come. *)
-   (own γ (● ((Excl' (), None), Some (to_agree false))) ∗
-        (∃ v, ℓ ↦ RESUMEDV v ∗ P v)) ∨
+   (own γ (● ((Excl' (), None), Some (to_agree false))) ∗ ℓ ↦ RESUMEDV ∗ P) ∨
    (* The reader came and broke the cannel; writer wasn't here. *)
    (own γ (● ((None, Excl' ()), Some (to_agree true))) ∗ ℓ ↦ CANCELLEDV) ∨
    (* Both have come; nothing interesting can happen now. *)
    (∃ (f: bool), own γ (● ((None, None), Some (to_agree f)))))%I.
 
 Definition is_asym_rendezvous γ v P :=
-  (∃ (ℓ: loc), ⌜v = #ℓ⌝ ∧ inv N (asym_rendezvous_inv P ℓ γ))%I.
+  (∃ (ℓ: loc), ⌜v = #ℓ⌝ ∧ inv N (asym_rendezvous_inv ℓ γ P))%I.
+
+Global Instance is_asym_rendezvous_persistent γ v P : Persistent (is_asym_rendezvous γ v P).
+Proof. apply _. Qed.
+
+Global Instance is_asym_rendezvous_inv_ne ℓ γ : NonExpansive (asym_rendezvous_inv ℓ γ).
+Proof. solve_proper. Qed.
+
+Global Instance is_asym_rendezvous_ne γ v : NonExpansive (is_asym_rendezvous γ v).
+Proof. solve_proper. Qed.
 
 Theorem init_exchange_spec ℓ P:
     {{{ ∃ v, ℓ ↦ v }}}
@@ -113,7 +122,7 @@ Proof.
   }
   repeat rewrite own_op.
   iDestruct "HOwn" as "[[HOwn Hfetch] Hpass]".
-  iMod (inv_alloc N _ (asym_rendezvous_inv P ℓ γ) with "[Hℓ HOwn]") as "HInv".
+  iMod (inv_alloc N _ (asym_rendezvous_inv ℓ γ P) with "[Hℓ HOwn]") as "HInv".
   {
     iNext. rewrite /asym_rendezvous_inv.
     eauto with iFrame.
@@ -125,35 +134,27 @@ Qed.
 Theorem await_spec γ r P:
     {{{ is_asym_rendezvous γ r P ∗ fetch_permit γ }}}
       await r
-    {{{ sm, RET sm; P sm ∗ passed γ }}}.
+    {{{ RET #(); P ∗ passed γ }}}.
 Proof.
   iIntros (Φ) "[#HIsR Hfp] HPost".
   iDestruct "HIsR" as (ℓ) "[% #HInv]". subst.
   iLöb as "IH". wp_lam. wp_bind (!_)%E.
   iInv N as "HInvO" "HInvC".
-  iDestruct "HInvO" as "[[>HOwn Hℓ]|[[>HOwn Hℓ]|[[>HOwn Hℓ]|H]]]".
+  iDestruct "HInvO" as "[[>HOwn Hℓ]|[[>HOwn [Hℓ HP]]|[[>HOwn Hℓ]|H]]]".
   - wp_load.
     iMod ("HInvC" with "[HOwn Hℓ]") as "_"; first by iLeft; iFrame.
     iModIntro.
     wp_pures.
     by iApply ("IH" with "Hfp").
-  - iDestruct "Hℓ" as (v) "[Hℓ HP]".
-    wp_load.
+  - wp_load.
     iMod (own_update_2 with "HOwn Hfp") as "[HOwn Hpassed]".
     {
       apply transitivity with (y:=(● (None, None, Some (to_agree false)))).
       - apply auth_update_dealloc.
-        apply local_update_unital_discrete.
-        intros z HValid HEq.
-        split; auto.
-        destruct z as [[z1 z2] z3]; simpl in *.
-        inversion HEq as [[HEq1 HEq2] HEq3]; simpl in *.
-        destruct z1.
-        {
-          inversion HEq1 as [x y HContra|]. subst.
-          inversion HContra.
-        }
-        done.
+        apply prod_local_update_1.
+        apply prod_local_update_1.
+        apply delete_option_local_update.
+        by apply excl_exclusive.
       - apply auth_update_core_id with (b := (None, None, Some (to_agree false))).
         apply pair_core_id; apply _.
         done.
@@ -167,51 +168,323 @@ Proof.
     wp_pures.
     iApply "HPost".
     iFrame.
-  - rewrite /fetch_permit.
-    iDestruct (own_valid_2 with "HOwn Hfp") as %HH.
-    apply auth_valid_discrete in HH; simpl in HH.
-    exfalso.
-    inversion HH as [_ [a [HAgr [HLe HVal]]]].
-    apply to_agree_inj in HAgr.
-    destruct a as [[u u'] u0].
-    inversion HAgr as [[HAgr' _] _].
-    inversion HAgr'; simpl in *; subst.
-    inversion HLe as [x [[HContra _] _]].
-    destruct x as [[xu xu'] xu0].
-    simpl in *.
-    destruct xu; by inversion HContra.
+  - iDestruct (own_valid_2 with "HOwn Hfp") as
+        %[[[[HContra|[a [b [_ [HContra _]]]]]%option_included _]
+             %prod_included _]
+            %prod_included _]
+         %auth_both_valid; discriminate.
   - iDestruct "H" as (f) ">HOwn".
-    rewrite /fetch_permit.
-    iDestruct (own_valid_2 with "HOwn Hfp") as %HH.
-    apply auth_valid_discrete in HH; simpl in HH.
-    exfalso.
-    inversion HH as [_ [a [HAgr [HLe HVal]]]].
-    apply to_agree_inj in HAgr.
-    destruct a as [[u u'] u0].
-    inversion HAgr as [[HAgr' _] _].
-    inversion HAgr'; simpl in *; subst.
-    inversion HLe as [x [[HContra _] _]].
-    destruct x as [[xu xu'] xu0].
-    simpl in *.
-    destruct xu; by inversion HContra.
+    iDestruct (own_valid_2 with "HOwn Hfp") as
+        %[[[[HContra|[a [b [_ [HContra _]]]]]%option_included _]
+             %prod_included _]
+            %prod_included _]
+         %auth_both_valid; discriminate.
 Qed.
 
-(*
-  await_interruptibly_spec Ni γi handle N γ r P:
+Lemma check_rendezvous_spec γ P ℓ :
+  {{{ inv N (asym_rendezvous_inv ℓ γ P) ∗ fetch_permit γ }}}
+    (λ: "e", !"e")%V #ℓ
+  {{{ (r: val), RET r; ⌜r = NONEV⌝ ∧ fetch_permit γ ∨
+                       ⌜r = RESUMEDV⌝ ∧ (fun (_: val) => P ∗ passed γ) #0 }}}.
+Proof.
+  iIntros (Φ) "[#HInv Hfp] HPost".
+  rewrite /asym_rendezvous_inv /fetch_permit.
+  wp_pures.
+  iInv N as "HInvO" "HInvC".
+  iDestruct "HInvO" as "[[>HOwn Hℓ]|[[>HOwn [Hℓ HP]]|[[>HOwn Hℓ]|H]]]".
+  - wp_load.
+    iMod ("HInvC" with "[HOwn Hℓ]") as "_"; first by eauto with iFrame.
+    iModIntro.
+    iApply "HPost".
+    by eauto with iFrame.
+  - iMod (own_update_2 with "HOwn Hfp") as "[HOwn HPassed]".
+    {
+      apply transitivity with (y := ● (None, None, Some (to_agree false))).
+      * apply auth_update_dealloc.
+        apply prod_local_update_1.
+        apply prod_local_update_1.
+        apply delete_option_local_update.
+        by apply excl_exclusive.
+      * apply auth_update_core_id with (b := (None, None, Some (to_agree false))).
+        apply pair_core_id; apply _.
+        done.
+    }
+    wp_load.
+    iMod ("HInvC" with "[HOwn Hℓ]") as "_"; first by eauto 10 with iFrame.
+    iModIntro.
+    iApply ("HPost" with "[HP HPassed]").
+    by eauto 10 with iFrame.
+  - iDestruct (own_valid_2 with "HOwn Hfp") as
+        %[[[[HContra|[a [b [_ [HContra _]]]]]%option_included _]
+             %prod_included _]
+            %prod_included _]
+         %auth_both_valid; discriminate.
+  - iDestruct "H" as (f) ">HOwn".
+    iDestruct (own_valid_2 with "HOwn Hfp") as
+        %[[[[HContra|[a [b [_ [HContra _]]]]]%option_included _]
+             %prod_included _]
+            %prod_included _]
+         %auth_both_valid; discriminate.
+Qed.
+
+Theorem await_interruptibly_spec Ni γi handle γ r P:
     {{{ is_interrupt_handle Ni γi handle ∗
-                            is_asym_rendezvous N γ r P ∗
+                            is_asym_rendezvous γ r P ∗
                             fetch_permit γ }}}
       await_interruptibly handle r
-    {{{ sm, RET sm; (∃ v, ⌜sm = (#false, RESUMEDV v)%V⌝ ∧ P v ∗ passed γ) ∨
-                    (∃ v, ⌜sm = (#true, RESUMEDV v)%V⌝ ∧ P v ∗ passed γ ∗
-                                                           interrupted γi) ∨
-                    (⌜sm = (#true, NONEV)%V⌝ ∧ cancelled γ)
-    }}};
-  pass_spec N γ r P v:
-    {{{ is_asym_rendezvous N γ r P ∗ pass_permit γ ∗ P v }}}
-      pass r v
+    {{{ sm, RET sm; ⌜sm = (#false, RESUMEDV)%V⌝ ∧ P ∗ passed γ ∨
+                    ⌜sm = (#true, RESUMEDV)%V⌝ ∧ ▷ P ∗ passed γ ∗ interrupted γi ∨
+                    ⌜sm = (#true, NONEV)%V⌝ ∧ cancelled γ
+    }}}.
+Proof.
+  iIntros (Φ) "[#HIsHandl [#HIsR Hfp]] HPost".
+  iDestruct "HIsR" as (ℓ) "[% #HInv]". subst.
+  rewrite /await_interruptibly /=.
+  wp_lam.
+  iApply (interruptibly_spec with "[Hfp]").
+  2: {
+    iNext.
+    iIntros (r v) "[[% Hx]|[% Hx]]"; subst; iApply ("HPost" with "[Hx]").
+    {
+      iRight.
+      instantiate (1:=(fun v => interrupted γi ∗
+                               ((⌜v = InjRV #false⌝ ∧ ▷ P ∗ passed γ)
+                                ∨ ⌜v = InjLV #()⌝ ∧ cancelled γ))%I).
+      simpl.
+      iDestruct "Hx" as "[HInt [[% [HP HPassed]]|[% HCan]]]"; subst; eauto.
+    }
+    {
+      iLeft.
+      instantiate (1:=(fun v => ⌜v = #false⌝ ∧ P ∗ passed γ)%I).
+      iDestruct "Hx" as "[% [HP HPassed]]".
+      subst; eauto with iFrame.
+    }
+  }
+  { iSplit; first done.
+    iSplitL; first by iApply "Hfp".
+    iSplit.
+    {
+      iModIntro.
+      iIntros (Φ') "Hfp HPost".
+      iApply (check_rendezvous_spec with "[Hfp]").
+      1: by iFrame.
+      iNext.
+      iIntros (r) "[HPre|[% [HP HPassed]]]"; iApply "HPost"; eauto 10.
+    }
+    {
+      iModIntro.
+      iIntros (Φ') "[Hfp #HIntr] HPost".
+      wp_lam.
+      wp_pures.
+      iClear "HIsHandl".
+      rewrite /fetch_permit.
+      awp_apply getAndSet.getAndSet_spec without "HPost".
+      iInv N as "HInvO".
+      iDestruct "HInvO" as "[[>HOwn Hℓ]|[[>HOwn [Hℓ HP]]|[[>HOwn Hℓ]|H]]]".
+      3: iDestruct (own_valid_2 with "HOwn Hfp") as
+            %[[[[HContra|[a [b [_ [HContra _]]]]]%option_included _]
+                %prod_included _]
+                %prod_included _]
+            %auth_both_valid; discriminate.
+      3: iDestruct "H" as (f) ">HOwn";
+        iDestruct (own_valid_2 with "HOwn Hfp") as
+            %[[[[HContra|[a [b [_ [HContra _]]]]]%option_included _]
+                %prod_included _]
+                %prod_included _]
+            %auth_both_valid; discriminate.
+      {
+        iAssert ((fun k => ▷ ℓ ↦ k ∧ ⌜val_is_unboxed k⌝) (InjLV #()))%I with "[Hℓ]" as "HII".
+        1: by iFrame.
+        iAaccIntro with "HII".
+        {
+          iIntros "[Hℓ _]".
+          iModIntro.
+          iFrame.
+          rewrite /asym_rendezvous_inv.
+          eauto 10 with iFrame.
+        }
+        {
+          iIntros "Hℓ".
+          iMod (own_update_2 with "HOwn Hfp") as "[HOwn HCancelled]".
+          {
+            apply transitivity with (y:= ● (None, Excl' (), None)).
+            - apply auth_update_dealloc.
+              apply prod_local_update_1.
+              apply prod_local_update_1.
+              apply delete_option_local_update.
+              apply excl_exclusive.
+            - apply auth_update_alloc with
+                  (b' := (None, None, Some (to_agree true))).
+              apply prod_local_update_2.
+              apply alloc_option_local_update.
+              done.
+          }
+          iModIntro.
+          iSplitL "Hℓ HOwn".
+          {
+            rewrite /asym_rendezvous_inv.
+            by eauto 10 with iFrame.
+          }
+          {
+            iIntros "HPost".
+            iApply "HPost".
+            eauto 10 with iFrame.
+          }
+        }
+      }
+      {
+        iAssert ((fun k => ▷ ℓ ↦ k ∧ ⌜val_is_unboxed k⌝) (InjRV #false))%I with "[Hℓ]" as "HII".
+        1: by iFrame.
+        iAaccIntro with "HII".
+        {
+          iIntros "[Hℓ _]".
+          iModIntro.
+          iFrame.
+          rewrite /asym_rendezvous_inv.
+          eauto 10 with iFrame.
+        }
+        {
+          iIntros "Hℓ".
+          iMod (own_update_2 with "HOwn Hfp") as "[HOwn HPassed]".
+          {
+            apply transitivity with (y := ● (None, None, Some (to_agree false))).
+            - apply auth_update_dealloc.
+              apply prod_local_update_1.
+              apply prod_local_update_1.
+              apply delete_option_local_update.
+              apply excl_exclusive.
+            - apply auth_update_core_id with (b := (None, None, Some (to_agree false))).
+              1: apply pair_core_id; by apply _.
+              done.
+          }
+          iModIntro.
+          iSplitR "HP HPassed".
+          2: {
+            iIntros "HPost".
+            iApply "HPost".
+            rewrite /passed.
+            iSplitR; eauto.
+          }
+          iNext.
+          rewrite /asym_rendezvous_inv.
+          eauto 10 with iFrame.
+        }
+      }
+    }
+  }
+Qed.
+
+Theorem pass_spec γ r P:
+    Laterable P ->
+    {{{ is_asym_rendezvous γ r P ∗ pass_permit γ ∗ P }}}
+      pass r
     {{{ sm, RET sm; ⌜sm = NONEV⌝ ∧ passed γ ∨
-                                    ⌜sm = CANCELLEDV⌝ ∧ P v ∗ cancelled γ}}}
-*)
+                    ⌜sm = CANCELLEDV⌝ ∧ P ∗ cancelled γ}}}.
+Proof.
+  iIntros (HLat Φ) "[#HIsR [Hpp HP]] HPost".
+  iDestruct "HIsR" as (ℓ) "[% #HInv]". subst.
+  rewrite /pass_permit.
+  wp_lam.
+  awp_apply getAndSet.getAndSet_spec without "HPost".
+  iInv N as "HInvO".
+  iDestruct "HInvO" as "[[>HOwn Hℓ]|[[>HOwn [Hℓ _]]|[[>HOwn Hℓ]|H]]]".
+  2: iDestruct (own_valid_2 with "HOwn Hpp") as
+      %[[[_ [HContra|[a [b [_ [HContra _]]]]]%option_included]
+           %prod_included _]
+          %prod_included _]
+       %auth_both_valid; discriminate.
+  3: {
+    iDestruct "H" as (f) ">HOwn".
+    iDestruct (own_valid_2 with "HOwn Hpp") as
+      %[[[_ [HContra|[a [b [_ [HContra _]]]]]%option_included]
+           %prod_included _]
+          %prod_included _]
+       %auth_both_valid; discriminate.
+  }
+  {
+    iAssert ((fun k => ▷ ℓ ↦ k ∧ ⌜val_is_unboxed k⌝) (InjLV #()))%I with "[Hℓ]" as "HII".
+    1: by iFrame.
+    iAaccIntro with "HII".
+    {
+      iFrame.
+      iIntros "[Hℓ _]".
+      iModIntro.
+      iNext.
+      rewrite /asym_rendezvous_inv.
+      eauto 10 with iFrame.
+    }
+    {
+      iIntros "Hℓ".
+      iMod (own_update_2 with "HOwn Hpp") as "[HOwn HPassed]".
+      {
+        apply transitivity with (y := ● (Excl' (), None, None)).
+        - apply auth_update_dealloc.
+          apply prod_local_update_1.
+          apply prod_local_update_2.
+          apply delete_option_local_update.
+          apply excl_exclusive.
+        - apply auth_update_alloc with (b' := (None, None, Some (to_agree false))).
+          apply prod_local_update_2.
+          apply alloc_option_local_update.
+          done.
+      }
+      iModIntro.
+      iSplitR "HPassed".
+      {
+        iNext.
+        rewrite /asym_rendezvous_inv.
+        eauto 10 with iFrame.
+      }
+      {
+        rewrite /passed.
+        iIntros "HPost".
+        iApply "HPost".
+        eauto.
+      }
+    }
+  }
+  {
+    iAssert ((fun k => ▷ ℓ ↦ k ∧ ⌜val_is_unboxed k⌝) (InjRV #true))%I with "[Hℓ]" as "HII".
+    1: by iFrame.
+    iAaccIntro with "HII".
+    {
+      iFrame.
+      iIntros "[Hℓ _]".
+      iModIntro.
+      iNext.
+      rewrite /asym_rendezvous_inv.
+      eauto 10 with iFrame.
+    }
+    {
+      iIntros "Hℓ".
+      iMod (own_update_2 with "HOwn Hpp") as "[HOwn HCancelled]".
+      {
+        apply transitivity with (y := ● (None, None, Some (to_agree true))).
+        - apply auth_update_dealloc.
+          apply prod_local_update_1.
+          apply prod_local_update_2.
+          apply delete_option_local_update.
+          apply excl_exclusive.
+        - apply auth_update_core_id with (b := (None, None, Some (to_agree true))).
+          { apply pair_core_id; apply _. }
+          done.
+      }
+      iModIntro.
+      iSplitR "HP HCancelled".
+      {
+        iNext.
+        rewrite /asym_rendezvous_inv.
+        eauto 10 with iFrame.
+      }
+      {
+        iIntros "HPost".
+        iApply "HPost".
+        rewrite /cancelled.
+        iRight.
+        eauto 10 with iFrame.
+      }
+    }
+  }
+Qed.
 
 End asym_rendezvous_proof.
